HoareArr.v
@@ -1,0 +1,684 @@
+
+(** * Hoare: Hoare Logic, Part II *)
+
+(***********************************************)
+(* Homework 1 Part 2: 
+   Define hoare logic rules for the ImpArr language,
+   complete the verification of a few programs using your rules.
+   There are 4 problems in this part.
+***********************************************)
+Require Export ImpArr.
+
+  
+(* ####################################################### *)
+(** * Hoare Logic *)
+
+(** Hoare Logic combines two beautiful ideas: a natural way of
+    writing down _specifications_ of programs, and a _compositional
+    proof technique_ for proving that programs are correct with
+    respect to such specifications -- where by "compositional" we mean
+    that the structure of proofs directly mirrors the structure of the
+    programs that they are about. *)
+
+(* ####################################################### *)
+(** ** Assertions *)
+
+(** To talk about specifications of programs, the first thing we
+    need is a way of making _assertions_ about properties that hold at
+    particular points during a program's execution -- i.e., claims
+    about the current state of the memory when program execution
+    reaches that point.  Formally, an assertion is just a family of
+    propositions indexed by a [state]. *)
+
+Definition Assertion := state -> Prop.
+
+Definition assert_implies (P Q : Assertion) : Prop :=
+  forall st, P st -> Q st.
+
+Notation "P ->> Q" :=
+  (assert_implies P Q) (at level 80) : hoare_spec_scope.
+
+Open Scope hoare_spec_scope.
+
+
+Notation "P <<->> Q" :=
+  (P ->> Q /\ Q ->> P) (at level 80) : hoare_spec_scope.
+
+
+Definition hoare_triple
+           (P:Assertion) (c:com) (Q:Assertion) : Prop :=
+  forall st st',
+       c / st || st'  ->
+       P st  ->
+       Q st'.
+
+Notation "{{ P }}  c  {{ Q }}" :=
+  (hoare_triple P c Q) (at level 90, c at next level)
+  : hoare_spec_scope.
+
+
+Theorem hoare_post_true : forall (P Q : Assertion) c,
+  (forall st, Q st) ->
+  {{P}} c {{Q}}.
+Proof.
+  intros P Q c H. unfold hoare_triple.
+  intros st st' Heval HP.
+  apply H.  Qed.
+
+Theorem hoare_pre_false : forall (P Q : Assertion) c,
+  (forall st, ~(P st)) ->
+  {{P}} c {{Q}}.
+Proof.
+  intros P Q c H. unfold hoare_triple.
+  intros st st' Heval HP.
+  unfold not in H. apply H in HP.
+  inversion HP.
+Qed.
+
+
+Definition assn_sub X a P : Assertion :=
+  fun (st : state) =>
+    P (update st X a).
+ 
+Notation "P [ X |-> a ]" := (assn_sub X a P) (at level 10).
+
+
+(** Now we can give the precise proof rule for assignment: 
+      ------------------------------ (hoare_asgn)
+      {{Q [X |-> a]}} X ::= a {{Q}}
+*)
+
+(** We can prove formally that this rule is indeed valid. *)
+(* The assignment rule is modified to take care of unsafe memory accesses *)
+Definition safe_aeval a n : Assertion :=
+ fun (st : state) => aeval st a = Some n.
+
+Theorem hoare_asgn : forall Q X a,
+  {{fun (st:state) => exists n, safe_aeval a n st /\ Q [X |-> n] st }}
+  (X ::= a)
+  {{Q}}.
+Proof.
+  unfold hoare_triple.
+  intros Q X a. intros st st' HE HQ.
+  destruct HQ as [n Hs].
+  destruct Hs as [Hsafe HQ].
+  inversion HE.  subst.
+  (* safe *)
+  unfold assn_sub in HQ. 
+   unfold safe_aeval in Hsafe.
+   assert (J: Some n = Some n0). 
+     congruence. 
+   inversion J; subst; assumption. 
+  (* core dump *)
+    unfold safe_aeval in Hsafe.
+   assert (J: Some n = None). congruence. 
+   inversion J.
+ Qed.
+
+
+(* ####################################################### *) 
+(** *** Consequence *)
+
+(** Sometimes the preconditions and postconditions we get from the
+    Hoare rules won't quite be the ones we want in the particular
+    situation at hand -- they may be logically equivalent but have a
+    different syntactic form that fails to unify with the goal we are
+    trying to prove, or they actually may be logically weaker (for
+    preconditions) or stronger (for postconditions) than what we need.
+
+    For instance, while
+      {{(X = 3) [X |-> 3]}} X ::= 3 {{X = 3}},
+    follows directly from the assignment rule, 
+      {{True}} X ::= 3 {{X = 3}}.
+    does not.  This triple is valid, but it is not an instance of
+    [hoare_asgn] because [True] and [(X = 3) [X |-> 3]] are not
+    syntactically equal assertions.  However, they are logically
+    equivalent, so if one triple is valid, then the other must
+    certainly be as well.  We might capture this observation with the
+    following rule:
+                {{P'}} c {{Q}}
+                  P <<->> P'
+         -----------------------------   (hoare_consequence_pre_equiv)
+                {{P}} c {{Q}}
+    Taking this line of thought a bit further, we can see that
+    strengthening the precondition or weakening the postcondition of a
+    valid triple always produces another valid triple. This
+    observation is captured by two _Rules of Consequence_.
+                {{P'}} c {{Q}}
+                   P ->> P'
+         -----------------------------   (hoare_consequence_pre)
+                {{P}} c {{Q}}
+
+                {{P}} c {{Q'}}
+                  Q' ->> Q 
+         -----------------------------    (hoare_consequence_post)
+                {{P}} c {{Q}}
+*)
+
+(** Here are the formal versions: *)
+
+Theorem hoare_consequence_pre : forall (P P' Q : Assertion) c,
+  {{P'}} c {{Q}} ->
+  P ->> P' ->
+  {{P}} c {{Q}}.
+Proof.
+  intros P P' Q c. intros Hhoare Himp.
+  intros st st' Hc HP. apply (Hhoare st st'). 
+  assumption. apply Himp. assumption.
+Qed.
+
+Theorem hoare_consequence_post : forall (P Q Q' : Assertion) c,
+  {{P}} c {{Q'}} ->
+  Q' ->> Q ->
+  {{P}} c {{Q}}.
+Proof.
+  intros P Q Q' c Hhoare Himp.
+  intros st st' Hc HP. 
+  apply Himp.
+  apply (Hhoare st st'). 
+  assumption. assumption.
+Qed.
+
+(** For example, we might use the first consequence rule like this:
+                {{ True }} ->>
+                {{ 1 = 1 }} 
+    X ::= 1
+                {{ X = 1 }}
+    Or, formally... 
+*)
+
+
+Theorem hoare_consequence : forall (P P' Q Q' : Assertion) c,
+  {{P'}} c {{Q'}} ->
+  P ->> P' ->
+  Q' ->> Q ->
+  {{P}} c {{Q}}.
+Proof.
+  intros P P' Q Q' c. intros Hht HPP' HQ'Q.
+  apply hoare_consequence_pre with (P' := P').
+  apply hoare_consequence_post with (Q' := Q').
+  assumption. assumption. assumption.  Qed.
+
+(* ####################################################### *)
+(** *** Skip *)
+
+(** Since [SKIP] doesn't change the state, it preserves any
+    property P:
+      --------------------  (hoare_skip)
+      {{ P }} SKIP {{ P }}
+*)
+
+Theorem hoare_skip : forall P,
+     {{P}} SKIP {{P}}.
+Proof.
+  intros P st st' H HP. inversion H. subst.
+  assumption.
+Qed.
+
+(* ####################################################### *) 
+(** *** Sequencing *)
+
+(** More interestingly, if the command [c1] takes any state where
+    [P] holds to a state where [Q] holds, and if [c2] takes any
+    state where [Q] holds to one where [R] holds, then doing [c1]
+    followed by [c2] will take any state where [P] holds to one
+    where [R] holds:
+        {{ P }} c1 {{ Q }} 
+        {{ Q }} c2 {{ R }}
+       ---------------------  (hoare_seq)
+       {{ P }} c1;;c2 {{ R }}
+*)
+
+Theorem hoare_seq : forall P Q R c1 c2,
+     {{Q}} c2 {{R}} ->
+     {{P}} c1 {{Q}} ->
+     {{P}} c1;;c2 {{R}}.
+Proof.
+  intros P Q R c1 c2. intros H2 H1. intros st st' H12 Pre.
+  inversion H12. subst.
+  apply (H2 st'0 st'). assumption.
+  apply (H1 st st'0). assumption.
+  apply Pre.
+Qed.
+
+(** Note that, in the formal rule [hoare_seq], the premises are
+    given in "backwards" order ([c2] before [c1]).  This matches the
+    natural flow of information in many of the situations where we'll
+    use the rule: the natural way to construct a Hoare-logic proof is
+    to begin at the end of the program (with the final postcondition)
+    and push postconditions backwards through commands until we reach
+    the beginning. *)
+
+(** Informally, a nice way of recording a proof using the sequencing
+    rule is as a "decorated program" where the intermediate assertion
+    [Q] is written between [c1] and [c2]:
+      {{ a = n }}
+    X ::= a;;
+      {{ X = n }}      <---- decoration for Q
+    SKIP
+      {{ X = n }}
+*)
+
+(* ####################################################### *) 
+(** *** Conditionals *)
+
+(** What sort of rule do we want for reasoning about conditional
+    commands?  Certainly, if the same assertion [Q] holds after
+    executing either branch, then it holds after the whole
+    conditional.  So we might be tempted to write:
+              {{P}} c1 {{Q}}
+              {{P}} c2 {{Q}}
+      --------------------------------
+      {{P}} IFB b THEN c1 ELSE c2 {{Q}}
+   However, this is rather weak. For example, using this rule,
+   we cannot show that:
+     {{ True }} 
+     IFB X == 0
+     THEN Y ::= 2
+     ELSE Y ::= X + 1 
+     FI
+     {{ X <= Y }}
+   since the rule tells us nothing about the state in which the
+   assignments take place in the "then" and "else" branches. *)
+   
+(** But we can actually say something more precise.  In the
+   "then" branch, we know that the boolean expression [b] evaluates to
+   [true], and in the "else" branch, we know it evaluates to [false].
+   Making this information available in the premises of the rule gives
+   us more information to work with when reasoning about the behavior
+   of [c1] and [c2] (i.e., the reasons why they establish the
+   postcondition [Q]). *)
+(**
+              {{P /\  b}} c1 {{Q}}
+              {{P /\ ~b}} c2 {{Q}}
+      ------------------------------------  (hoare_if)
+      {{P}} IFB b THEN c1 ELSE c2 FI {{Q}} 
+*)
+
+
+(** Now we can formalize the Hoare proof rule for conditionals
+    and prove it correct. *)
+Definition safe_beval b n : Assertion :=
+ fun (st : state) => beval st b = Some n.
+
+Theorem hoare_if : forall P Q b c1 c2,
+  {{fun st => P st /\ safe_beval b true st}} c1 {{Q}} ->
+  {{fun st => P st /\ safe_beval b false st}} c2 {{Q}} ->
+  {{fun st => P st /\ exists n, safe_beval b n st}} 
+    (IFB b THEN c1 ELSE c2 FI) {{Q}}.
+Proof.
+  intros P Q b c1 c2. intros HTrue HFalse. intros st st' Hcommand HPre.
+  destruct HPre as [HP HE].
+  inversion Hcommand. subst.
+  Case "b = true". apply (HTrue st st'). assumption.
+  split. assumption. assumption.
+  Case "b = false". apply (HFalse st st'). assumption.
+  split. assumption. assumption.
+  Case "beval st b = None".
+  destruct HE as [n HE']. unfold safe_beval in HE'.
+  assert (J : None = Some n). congruence.
+  inversion J.
+Qed.
+
+
+
+
+(* ####################################################### *) 
+
+(* ####################################################### *)
+(** *** Loops *)
+
+(** Finally, we need a rule for reasoning about while loops. *)
+
+(** Suppose we have a loop
+      WHILE b DO c END
+    and we want to find a pre-condition [P] and a post-condition
+    [Q] such that
+      {{P}} WHILE b DO c END {{Q}} 
+    is a valid triple. *)
+
+(** *** *)
+
+(** First of all, let's think about the case where [b] is false at the
+    beginning -- i.e., let's assume that the loop body never executes
+    at all.  In this case, the loop behaves like [SKIP], so we might
+    be tempted to write: *)
+
+(**
+      {{P}} WHILE b DO c END {{P}}.
+*)
+
+(** 
+    But, as we remarked above for the conditional, we know a
+    little more at the end -- not just [P], but also the fact
+    that [b] is false in the current state.  So we can enrich the
+    postcondition a little:
+*)
+(** 
+      {{P}} WHILE b DO c END {{P /\ ~b}}
+*)
+
+(** 
+    What about the case where the loop body _does_ get executed?
+    In order to ensure that [P] holds when the loop finally
+    exits, we certainly need to make sure that the command [c]
+    guarantees that [P] holds whenever [c] is finished.
+    Moreover, since [P] holds at the beginning of the first
+    execution of [c], and since each execution of [c]
+    re-establishes [P] when it finishes, we can always assume
+    that [P] holds at the beginning of [c].  This leads us to the
+    following rule:
+*)
+(** 
+                   {{P}} c {{P}}
+        -----------------------------------  
+        {{P}} WHILE b DO c END {{P /\ ~b}}
+*)
+(** 
+    This is almost the rule we want, but again it can be improved a
+    little: at the beginning of the loop body, we know not only that
+    [P] holds, but also that the guard [b] is true in the current
+    state.  This gives us a little more information to use in
+    reasoning about [c] (showing that it establishes the invariant by
+    the time it finishes).  This gives us the final version of the rule:
+*)
+(**
+               {{P /\ b}} c {{P}}
+        -----------------------------------  (hoare_while)
+        {{P}} WHILE b DO c END {{P /\ ~b}}
+    The proposition [P] is called an _invariant_ of the loop.
+ *)
+
+
+Lemma safe_bexp_eval_false : forall b st,
+  beval st b = Some false -> (safe_beval b false) st.
+Proof.
+  intros. unfold safe_beval. assumption.
+Qed.
+
+Lemma safe_bexp_eval_true: forall b st,
+  beval st b = Some true -> (safe_beval b true) st.
+Proof.
+  intros. unfold safe_beval. assumption.
+Qed.
+
+(**********************************************
+
+  Homework 2.1: complete the following proof. 
+ 
+ ***********************************************)
+Lemma hoare_while : forall P b c,
+  (P ->> (fun st => exists n, safe_beval b n st)) -> 
+  {{fun st => P st /\ safe_beval b true st}} c {{P}} ->
+  {{fun st => P st }}
+  WHILE b DO c END 
+  {{fun st => P st /\ safe_beval b false st}}.
+Proof. 
+  intros P b c. intros Hs Hpre. intros st st' HCommand HPre.
+  remember (WHILE b DO c END) as wcom eqn:Heqwcom.
+  ceval_cases (induction HCommand) Case;
+    try (inversion Heqwcom); subst; clear Heqwcom.
+  Case "E_WhileEnd".
+  split. assumption. apply safe_bexp_eval_false. assumption.
+  Case "E_WhileLoop".
+  apply IHHCommand2. reflexivity.
+  apply (Hpre st st'). assumption.
+  split. assumption. apply safe_bexp_eval_true. assumption.
+  Case "E_While_fail".
+  split.
+  apply Hs in HPre; destruct HPre as [n HPre'];
+  unfold safe_beval in HPre';
+  assert (J : Some n = None); congruence; inversion J.
+  apply Hs in HPre. destruct HPre as [n HPre'].
+  unfold safe_beval in HPre'.
+  assert (J : Some n = None). congruence. inversion J.
+Qed.
+ 
+  
+
+Definition undef_aeval a : Assertion :=
+ fun (st : state) => aeval st a = None.
+
+Definition unalloc_aeval a : Assertion :=
+ undef_aeval (ALen a).
+
+(**********************************************
+
+  Homework 2.2: Define the hoare triple for alloc
+  and prove it correct
+ 
+ ***********************************************)
+
+Definition update_none (st : state) (x : id) : state :=
+ match st with
+   | Safe st' => Safe (fun x' => if eq_id_dec x x' then None else st' x')
+   | CoreDump => CoreDump
+ end.
+
+Theorem hoare_new: forall arr a Q, 
+    {{fun (st:state) =>
+        exists n, safe_aeval a n st /\ Q (update st (Idx arr 0) n)
+        /\ aeval st (ALen arr) = None}}
+ ALLOC arr [[a]]
+ {{Q}}.
+Proof.
+  intros arr a Q. intros st st' Hc HPre.
+  destruct HPre as [n HPre'].
+  destruct HPre' as [HP1 HP23].
+  destruct HP23 as [HP2 HP3].
+  inversion Hc. subst.
+  unfold safe_aeval in HP1.
+  assert (H : Some n = Some n0). congruence.
+  inversion H. rewrite <- H2. assumption.
+  Case "coredump".
+  destruct H3 as [H3A | H3B]. subst.
+  unfold safe_aeval in HP1.
+  assert (J : Some n = None). congruence. inversion J.
+  destruct H3B as [i H3B']. subst.
+  assert (J : Some i = None). congruence. inversion J.
+Qed.
+
+
+
+Theorem hoare_new_abort: forall arr a Q, 
+    {{fun (st:state) =>
+        exists n, safe_aeval a n st /\ aeval st (ALen arr) = None }}
+ ALLOC arr [[a]]
+ {{Q}}.
+Proof.
+  intros arr a Q. intros st st' Hc HPre.
+  destruct HPre as [n HPre'].
+  destruct HPre' as [HP1 HP2].
+  inversion Hc. subst.
+  unfold safe_aeval in HP1. admit.
+  Case "coredump".
+  destruct H3 as [H3A | H3B]. subst.
+  unfold safe_aeval in HP1.
+  assert (J : Some n = None). congruence. inversion J.
+  destruct H3B as [i H3B'].
+  assert (J : Some n = None). congruence. inversion J.
+Qed.
+  
+  
+  
+  
+
+(**********************************************
+
+  Homework 2.3: Define the hoare triple for write
+  and prove it correct
+ 
+ ***********************************************)
+Theorem hoare_write : forall Q  a i x,
+    {{fun (st:state) =>
+        exists m, safe_aeval x m st /\
+        exists n, safe_aeval i n st /\
+        Q [(Idx a n) |-> m] st }} 
+  (WRITE a [[i]] x)
+  {{Q}}.
+Proof.
+  intros Q a i x. intros st st' Hcommand HPre.
+  destruct HPre as [m' HPre']. destruct HPre' as [H1 H23].
+  destruct H23 as [n' H23']. destruct H23' as [H2 H3].
+  inversion Hcommand. subst.
+  Case "safe_aeval i n".
+  unfold assn_sub in H3.
+  unfold safe_aeval in H1. unfold safe_aeval in H2.
+  assert (SameM : m' = m). congruence.
+  assert (SameN : n' = n). congruence.
+  rewrite <- SameM. rewrite <- SameN. apply H3.
+  Case "CoreDump".
+  subst. unfold assn_sub in H3.
+  destruct H7 as [Hinone | Hxnone].
+  unfold safe_aeval in H2.
+  assert (J : Some n' = None). congruence. inversion J.
+  unfold safe_aeval in H1.
+  assert (J : Some m' = None). congruence. inversion J.
+Qed.
+  
+  
+
+
+Definition prog1 :=  
+(ALLOC A [[ANum 10]]);;
+(ALLOC A [[ANum 20]]).
+
+Definition crash st := st = CoreDump.
+
+(* A few execises to test your new rules *)
+Lemma hoare_prog1: 
+ {{fun st => st =  empty_state}} prog1 
+{{crash}}.
+Proof. 
+ Admitted.
+
+Definition safe st := exists st', st = Safe st'.
+Definition prog2 :=  
+(ALLOC A [[ANum 10]]);;
+(WRITE A [[ANum 9]] ANum 9).
+
+Lemma hoare_prog2: 
+ {{fun st => st = empty_state}} prog2 
+{{safe}}.
+Proof. 
+ Admitted. 
+
+Definition prog3 :=  
+(ALLOC A [[ANum 10]]);;
+(WRITE A [[ANum 11]] ANum 9).
+
+Lemma hoare_prog3: 
+ {{fun st => st = empty_state}} prog3
+{{crash}}.
+Proof. 
+ Admitted. 
+
+(**********************************************
+
+  Homework 2.4: Analyze the following program.
+ This program mimics a protocol that acquires and releases locks of resources.
+ The locks to resources are represented as an array. 
+ The first loop initialized all locks to be unlocked (set to 0).
+ The second loop acquires all locks by setting all array elements to 1. 
+ The last loop releases all locks by decrementing all array elements by 1. 
+ 
+ ***********************************************)
+Definition prog4 : com := 
+  Z ::= ANum 10;;
+  (ALLOC A [[AId Z]]);;
+  Y ::= (ANum 1);;
+  WHILE (BLe (AId Y) (AId Z)) DO
+    (WRITE A [[AId Y]] (ANum 0));;
+   Y ::= APlus (AId Y) (ANum 1) 
+  END;; 
+  Y ::= (ANum 1);;
+  WHILE (BLe (AId Y) (AId Z)) DO
+    (WRITE A [[AId Y]] (ANum 1));;
+   Y ::= APlus (AId Y) (ANum 1) 
+  END;;
+  Y ::= (AId Z);;
+  WHILE (BLe (ANum 1) (AId Y) ) DO
+    (WRITE A [[AId Y]] (AMinus (AArr A (AId Y)) (ANum 1)));;
+   Y ::= AMinus (AId Y) (ANum 1) 
+  END.
+
+(* We need inductively defined properties for our analysis *)
+
+(* all_zero st A n means that all elements of A up to n are 0 *)
+Inductive all_zero: state -> id -> nat -> Prop :=
+| All_zero_base: forall st a, all_zero st a 0
+| All_zero_succ: forall st a n,
+    aeval st (AArr a (ANum (S n)))= Some 0 -> all_zero st a n ->
+    all_zero st a (S n).
+
+Inductive all_one: state -> id -> nat -> Prop :=
+| All_one_base: forall st a, all_one st a 0
+| All_one_succ: forall st a n,
+    aeval st (AArr a (ANum (S n)))= Some 1 -> all_one st a n ->
+    all_one st a (S n).
+
+Print empty_state.
+
+(* Prove the following Hoare triple. 
+   You may need to define your own inductive properties. *)
+Lemma hoare_prog4 :
+ {{fun st => st = empty_state}}
+ prog4
+ {{fun st =>exists n, aeval st (ALen A) = Some n /\ all_zero st A n}}.
+Proof. 
+  eapply hoare_seq. eapply hoare_seq. eapply hoare_seq. eapply hoare_seq.
+  eapply hoare_seq. eapply hoare_seq. eapply hoare_seq.
+  eapply hoare_consequence_post.
+  apply hoare_while.
+  Case "loop body preserves invariant".
+  intros st H.
+  apply H.
+  unfold hoare_triple. intros.
+  destruct H0 as [H1 H2].
+  destruct H1 as [n H1']. exists n. 
+  Abort.
+  
+  
+
+
+  
+(* ####################################################### *)
+(** ** Complete List of Hoare Logic Rules *)
+
+(** Above, we've introduced Hoare Logic as a tool to reasoning
+    about Imp programs. In the reminder of this chapter we will
+    explore a systematic way to use Hoare Logic to prove properties
+    about programs. The rules of Hoare Logic are the following: *)
+
+(**
+             ------------------------------ (hoare_asgn)
+             {{Q [X |-> a]}} X::=a {{Q}}
+
+             --------------------  (hoare_skip)
+             {{ P }} SKIP {{ P }}
+
+               {{ P }} c1 {{ Q }} 
+               {{ Q }} c2 {{ R }}
+              ---------------------  (hoare_seq)
+              {{ P }} c1;;c2 {{ R }}
+
+              {{P /\  b}} c1 {{Q}}
+              {{P /\ ~b}} c2 {{Q}}
+      ------------------------------------  (hoare_if)
+      {{P}} IFB b THEN c1 ELSE c2 FI {{Q}} 
+
+               {{P /\ b}} c {{P}}
+        -----------------------------------  (hoare_while)
+        {{P}} WHILE b DO c END {{P /\ ~b}}
+
+                {{P'}} c {{Q'}}
+                   P ->> P'
+                   Q' ->> Q
+         -----------------------------   (hoare_consequence)
+                {{P}} c {{Q}}
+    In the next chapter, we'll see how these rules are used to prove
+    that programs satisfy specifications of their behavior.
+*)
+
+(** $Date: 2014-12-31 11:17:56 -0500 (Wed, 31 Dec 2014) $ *)
+
