ImpArr.v
@@ -1,0 +1,517 @@
+(** * Based on Imp: Simple Imperative Programs *)
+(** * Based on ImpArr adds to the state arrays *)
+
+Require Export SfLib.
+
+(* ##################################################### *)
+(** ** Identifiers *)
+
+(** To begin, we'll need to formalize _identifiers_ such as program
+    variables.  We could use strings for this -- or, in a real
+    compiler, fancier structures like pointers into a symbol table.
+    But for simplicity let's just use natural numbers as identifiers. *)
+
+(** (We hide this section in a module because these definitions are
+    actually in [SfLib], but we want to repeat them here so that we
+    can explain them.) *)
+
+(** We define a new inductive datatype [Id] so that we won't confuse
+    identifiers and numbers.  We use [sumbool] to define a computable
+    equality operator on [Id]. *)
+
+(* "Id n" represents a variable *)
+(* "Idx a n" represents the nth element of array a *)
+Inductive id : Type :=
+ | Id : nat -> id
+ | Idx : id -> nat -> id. (* <--- new for array*)
+
+
+Theorem eq_id_dec : forall id1 id2 : id, {id1 = id2} + {id1 <> id2}.
+Proof. 
+   intro id1.  
+   induction id1; intro id2; destruct id2 as [n21 | n22].
+   destruct (eq_nat_dec n n21) as [Heq | Hneq].
+   Case "Id n1 = Id n2".
+     left. rewrite Heq. reflexivity.
+   Case "Id n1 <> Id n2".
+     right. intros contra. inversion contra. apply Hneq. apply H0.
+  Case "Id n1 <> Idx n2".
+     right. intros contra. inversion contra. 
+  Case "Idx n1 <> Id n2".
+     right. intros contra. inversion contra. 
+
+  destruct (IHid1 n22) as [Heq | Hneq]. 
+     destruct (eq_nat_dec n n0) as [Heqi | Hneqi].
+  Case "Idx n1 = Idx n2".
+    left; subst; auto.
+   Case "Idx n n1 <> Idx n n2".
+     right; intro J; inversion J; subst; apply Hneqi; auto.
+  Case "Idx n1 n <> Idx n2 n".
+     right; intro J; inversion J; subst; apply Hneq; auto.
+Qed.
+(*Defined. *)
+
+
+(** The following lemmas will be useful for rewriting terms involving [eq_id_dec]. *)
+
+Lemma eq_id : forall (T:Type) x (p q:T), 
+              (if eq_id_dec x x then p else q) = p. 
+Proof.
+  intros. 
+  destruct (eq_id_dec x x). 
+  Case "x = x". 
+    reflexivity.
+  Case "x <> x (impossible)". 
+  apply ex_falso_quodlibet. apply n. reflexivity.
+Qed.
+
+Lemma neq_id : forall (T:Type) x y (p q:T), x <> y -> 
+               (if eq_id_dec x y then p else q) = q. 
+Proof.
+ intros. 
+ destruct (eq_id_dec x y).
+ contradiction. (* assert (J:= H e).  inversion J. *)
+ reflexivity.
+Qed.
+(** [] *)
+
+
+(* End Id. *)
+
+(* ####################################################### *)
+(** ** States *)
+ 
+(** A _state_ represents the current values of _all_ the variables at
+    some point in the execution of a program. *)
+(** For simplicity (to avoid dealing with partial functions), we
+    let the state be defined for _all_ variables, even though any
+    given program is only going to mention a finite number of them. 
+    The state captures all of the information stored in memory.  For Imp
+    programs, because each variable stores only a natural number, we
+    can represent the state as a mapping from identifiers to [nat].  
+    For more complex programming languages, the state might have more 
+    structure.  
+*)
+
+(* We distinguish between a well-formed state and a crashed state.
+   CoreDump results from unsafe access to the state 
+   such as double allocation and out of bounds access.
+
+   We assume the A[0] stores the length of array A. 
+   Accesses to A[i] where 0< A < A[0]+1 is safe
+*)
+
+Inductive state :=
+| Safe: (id -> option nat) -> state
+| CoreDump: state. 
+
+Definition empty_state : state :=
+  Safe (fun _ => None ).
+
+(* read returns (Some n) if the access is safe 
+   and x is mapped to n in the state; 
+   returns None otherwise
+*)
+Definition read (st: state) (x: id) : option nat :=
+ match st with
+ | Safe st' =>       
+   match x with 
+     | Idx a 0 => st' x
+     | Idx a (S i) => 
+        (match st' (Idx a 0) with
+           | Some b =>  
+             if (ble_nat i b) then st' x
+             else None
+           | None => None
+         end)
+     | _ => st' x
+   end
+ | CoreDump => None
+ end.
+
+(* update returns a new Safe state if the write is safe; 
+   returns CoreDump otherwise
+*)
+Definition update (st : state) (x : id) (n : nat) : state :=
+ match st with
+   | Safe st' => 
+     match x with
+       | Idx a 0 =>  
+          match st' (Idx a 0) with
+              | Some _ => CoreDump
+              | None =>
+                Safe (fun x' => if eq_id_dec x x' then Some (n) else st' x')
+          end
+       | Idx a (S i) => 
+         match st' (Idx a 0) with
+              | Some m => 
+                if (ble_nat (S i) m) then 
+                  Safe (fun x' => if eq_id_dec x x' then Some (n) else st' x')
+                else CoreDump
+              | None => CoreDump
+         end
+       | _ => Safe (fun x' => if eq_id_dec x x' then Some (n) else st' x')
+     end
+ | CoreDump => CoreDump
+ end.
+   
+
+Theorem update_eq1 : forall n x st,
+  read (update (Safe st) (Id x) n) (Id x) = Some n.
+Proof.
+  intros. 
+  unfold update. unfold read. apply eq_id.
+Qed.
+(** [] *)
+
+
+Theorem update_neq1 : forall x2 x1 n st,
+  Id x2 <> Id x1 ->                        
+  read (update st (Id x2) n) (Id x1) = read st (Id x1).
+Proof.
+intros. 
+  unfold update; unfold read. 
+ destruct st; simpl.
+ apply neq_id. apply H.
+ reflexivity.
+Qed.
+
+
+
+(* ################################################### *)
+(** ** Syntax  *)
+
+(** We can add variables to the arithmetic expressions we had before by
+    simply adding one more constructor: *)
+
+(* array element A[i] is encoded as AArr A (ANum i)
+   ALen A evaluates to the length of A, which is stored at A[0]
+ *)
+
+Inductive aexp : Type :=
+  | ANum : nat -> aexp
+  | AId : id -> aexp               
+  | AArr : id -> aexp -> aexp  (*<-- new *)             
+  | ALen : id -> aexp (*<-- nw *)
+  | APlus : aexp -> aexp -> aexp
+  | AMinus : aexp -> aexp -> aexp
+  | AMult : aexp -> aexp -> aexp.
+
+Tactic Notation "aexp_cases" tactic(first) ident(c) :=
+  first;
+  [ Case_aux c "ANum" | Case_aux c "AId" 
+  | Case_aux c "AArr" | Case_aux c "ALen"  | Case_aux c "APlus"
+  | Case_aux c "AMinus" | Case_aux c "AMult" ].
+
+(** Defining a few variable names as notational shorthands will make
+    examples easier to read: *)
+
+Definition X : id := Id 0.
+Definition Y : id := Id 1.
+Definition Z : id := Id 2.
+
+(**  definition a few arrays. 
+    These can be viewed as global variables **)
+Definition A : id := Id 3.
+Definition B : id := Id 4.
+Definition C : id := Id 5.
+
+
+(** The definition of [bexp]s is the same as before (using the new
+    [aexp]s): *)
+
+Inductive bexp : Type :=
+  | BTrue : bexp
+  | BFalse : bexp
+  | BEq : aexp -> aexp -> bexp
+  | BLe : aexp -> aexp -> bexp
+  | BNot : bexp -> bexp
+  | BAnd : bexp -> bexp -> bexp.
+
+Tactic Notation "bexp_cases" tactic(first) ident(c) :=
+  first;
+  [ Case_aux c "BTrue" | Case_aux c "BFalse" | Case_aux c "BEq"
+  | Case_aux c "BLe" | Case_aux c "BNot" | Case_aux c "BAnd" ].
+
+(* ################################################### *)
+(** ** Evaluation  *)
+
+(** The arith and boolean evaluators can be extended to handle
+    variables in the obvious way: *)
+
+Fixpoint aeval (st : state) (a : aexp) : option nat :=
+  match a with
+  | ANum n => Some n
+  | AId x => read st x                                  
+  | AArr x a => match (aeval st a) with 
+                | Some n => read st (Idx x n)
+                | None => None
+              end
+     (* <----- NEW *)
+  | ALen x => read st (Idx x 0)
+     (* <----- NEW *)
+  | APlus a1 a2 => match ( (aeval st a1), (aeval st a2)) with
+                     |(Some b1, Some b2) => Some (b1 + b2)
+                     | _ => None
+                   end
+  | AMinus a1 a2  => match ( (aeval st a1), (aeval st a2)) with
+                     |(Some b1, Some b2) => Some (b1 - b2)
+                     | _ => None
+                     end
+  | AMult a1 a2 =>  match ( (aeval st a1), (aeval st a2)) with
+                     |(Some b1, Some b2) => Some (b1 * b2)
+                     | _ => None
+                    end
+  end.
+
+Fixpoint beval (st : state)  (b : bexp) : option bool :=
+  match b with
+  | BTrue       => Some true
+  | BFalse      => Some false
+  | BEq a1 a2   => match ( (aeval st a1), (aeval st a2)) with
+                     |(Some b1, Some b2) => Some (beq_nat b1 b2)
+                     | _ => None
+                   end 
+  | BLe a1 a2   => match ( (aeval st a1), (aeval st a2)) with
+                     |(Some b1, Some b2) => Some (ble_nat b1 b2)
+                     | _ => None
+                   end 
+  | BNot b1     => match (beval st b1) with
+                     | Some b2 => Some (negb b2)
+                     | _ => None
+                   end 
+  | BAnd b1 b2  => match ( (beval st b1), (beval st b2)) with 
+                     |(Some b3, Some b4) => Some (andb b3 b4)
+                     | _ => None
+                   end 
+  end.
+
+
+(* the commands are updated to include array allocation and update 
+   CWrite A i e updates the ith element of A by e.
+   CAlloc A n allocates n cells for array A.
+   allocation can be done only once for each array.
+*)
+
+Inductive com : Type :=
+  | CSkip : com
+  | CAss : id -> aexp -> com
+  | CSeq : com -> com -> com
+  | CIf : bexp -> com -> com -> com
+  | CWhile : bexp -> com -> com
+  | CWrite : id -> aexp -> aexp -> com (*<-- New *)
+  | CAlloc: id -> aexp -> com (*<-- New *)
+.
+
+Tactic Notation "com_cases" tactic(first) ident(c) :=
+  first;
+  [ Case_aux c "SKIP" | Case_aux c "::=" | Case_aux c ";;"
+  | Case_aux c "IFB" | Case_aux c "WHILE" | Case_aux c "WRITE" | Case_aux c "ALLOC" ].
+
+(** As usual, we can use a few [Notation] declarations to make things
+    more readable.  We need to be a bit careful to avoid conflicts
+    with Coq's built-in notations, so we'll keep this light -- in
+    particular, we won't introduce any notations for [aexps] and
+    [bexps] to avoid confusion with the numerical and boolean
+    operators we've already defined.  We use the keyword [IFB] for
+    conditionals instead of [IF], for similar reasons. *)
+
+Notation "'SKIP'" :=
+  CSkip.
+Notation "x '::=' a" :=
+  (CAss x a) (at level 60).
+Notation "c1 ;; c2" :=
+  (CSeq c1 c2) (at level 80, right associativity).
+Notation "'WHILE' b 'DO' c 'END'" :=
+  (CWhile b c) (at level 80, right associativity).
+Notation "'IFB' c1 'THEN' c2 'ELSE' c3 'FI'" :=
+  (CIf c1 c2 c3) (at level 80, right associativity).
+Notation "'WRITE' a1 '[[' a2 ']]' a3"  :=
+  (CWrite a1 a2 a3) (at level 100).
+Notation "'ALLOC' i '[[' a ']]'"  :=
+  (CAlloc i a) (at level 79 , right associativity).
+
+(** For example, here is the factorial function again, written as a
+    formal definition to Coq: *)
+
+Definition loop : com := 
+  (ALLOC X [[ANum 10]]);;
+  Y ::= (ANum 0);;
+  WHILE (BLe (AId Y) (ANum 10)) DO
+   WRITE X[[AId Y]] (AId Y)
+  END.
+
+(* ################################################################ *)
+(** * Evaluation *)
+
+(** Next we need to define what it means to evaluate an Imp command.
+    The fact that [WHILE] loops don't necessarily terminate makes defining
+    an evaluation function tricky... *)
+
+(* #################################### *)
+(** ** Evaluation as a Relation *)
+
+(** Here's a better way: we define [ceval] as a _relation_ rather than
+    a _function_ -- i.e., we define it in [Prop] instead of [Type], as
+    we did for [aevalR] above. *)
+
+(** This is an important change.  Besides freeing us from the awkward
+    workarounds that would be needed to define evaluation as a
+    function, it gives us a lot more flexibility in the definition.
+    For example, if we added concurrency features to the language,
+    we'd want the definition of evaluation to be non-deterministic --
+    i.e., not only would it not be total, it would not even be a
+    partial function! *)
+(** We'll use the notation [c / st || st'] for our [ceval] relation:
+    [c / st || st'] means that executing program [c] in a starting
+    state [st] results in an ending state [st'].  This can be
+    pronounced "[c] takes state [st] to [st']".
+
+*)
+
+(** Here is the formal definition.  (Make sure you understand
+    how it corresponds to the inference rules.) *)
+
+Reserved Notation "c1 '/' st '||' st'" 
+ (at level 40, st at level 39).
+(* the evaluation relations are augmented with new rules to handle 
+   array operations and unsafe memory accesses*)
+
+Inductive ceval : com -> state -> state -> Prop :=
+  | E_Skip : forall st,
+      SKIP / st || st
+  | E_Ass_s  : forall st a1 n x,
+      aeval st a1 = Some n ->
+      (x ::= a1) / st || update st x n
+  | E_Ass_f  : forall st a1 x,
+      aeval st a1 = None ->
+      (x ::= a1) / st || CoreDump
+  (*<-- NEW 
+    if a1 evaluates to None, which indicates this is an unsafe access,
+    the state crashes
+   *)
+ | E_Seq : forall c1 c2 st st' st'',
+      c1 / st  || st' ->
+      c2 / st' || st'' ->
+      (c1 ;; c2) / st || st''
+  | E_IfTrue : forall st st' b c1 c2,
+      beval st b = Some true ->
+      c1 / st || st' ->
+      (IFB b THEN c1 ELSE c2 FI) / st || st'
+  | E_IfFalse : forall st st' b c1 c2,
+      beval st b = Some false ->
+      c2 / st || st' ->
+      (IFB b THEN c1 ELSE c2 FI) / st|| st'
+ | E_If_f : forall st  b c1 c2,
+      beval st b = None ->
+      (IFB b THEN c1 ELSE c2 FI) / st|| CoreDump
+  (* <-- New *)
+  | E_WhileEnd : forall b st c,
+      beval st b = Some false ->
+      (WHILE b DO c END) / st || st
+  | E_WhileLoop : forall st st' st'' b c,
+      beval st b = Some true ->
+      c / st || st' ->
+      (WHILE b DO c END) / st' || st'' ->
+      (WHILE b DO c END) / st || st''
+  | E_While_f : forall b st c,
+      beval st b = None ->
+      (WHILE b DO c END) / st || CoreDump
+  (* <-- New *)
+   | E_Alloc: forall st size n a,
+       aeval st size = Some n ->
+       aeval st (ALen a) = None ->
+      (ALLOC a [[size]]) / st ||  update st (Idx a 0) n
+   (* when allocating memory for an array, 
+      we check that the size expression can be evaluated, 
+      and that the array has not been allocated before. 
+      The size of the array is written to the 0th element *)
+  | E_Alloc_f: forall st size a ,
+       aeval st size = None \/  (exists i, aeval st (ALen a) = Some i)->
+      (ALLOC a [[size]]) / st ||  CoreDump
+   | E_Write: forall st x n m a b,
+       aeval st x = Some n ->
+       aeval st b = Some m -> 
+      (WRITE a [[x]] b) / st || update  st (Idx a n) m
+   (* the update function returns CoreDump for all unsafe accesess*)
+  | E_Write_f: forall st x a b,
+      (aeval st x = None \/ 
+       aeval st b = None) -> 
+       (WRITE a [[x]] b) / st || CoreDump
+
+  where "c1 '/' st '||' st'" := (ceval c1 st st').
+
+
+
+
+Tactic Notation "ceval_cases" tactic(first) ident(c) :=
+  first;
+  [ Case_aux c "E_Skip" | Case_aux c "E_Ass_s" | Case_aux c "E_Ass_fail" 
+    | Case_aux c "E_Seq"| Case_aux c "E_IfTrue" | Case_aux c "E_IfFalse"
+    | Case_aux c "E_If_fail" | Case_aux c "E_WhileEnd" 
+    | Case_aux c "E_WhileLoop" |Case_aux c "E_While_fail"
+    | Case_aux c "E_Alloc" |Case_aux c "E_Alloc_fail"
+    | Case_aux c "E_Write" |Case_aux c "E_Write_fail"
+ ].
+
+(** *** *)
+(** The cost of defining evaluation as a relation instead of a
+    function is that we now need to construct _proofs_ that some
+    program evaluates to some result state, rather than just letting
+    Coq's computation mechanism do it for us. *)
+
+Example ceval_example1:
+    (X ::= ANum 2;;
+     IFB BLe (AId X) (ANum 1)
+       THEN Y ::= ANum 3
+       ELSE Z ::= ANum 4
+     FI)
+   / empty_state
+   || (update (update empty_state X 2) Z 4).
+Proof.
+  (* We must supply the intermediate state *)
+  apply E_Seq  with (update empty_state X 2).
+  Case "assignment command".
+    apply E_Ass_s. reflexivity.
+    Case "if command".
+    apply E_IfFalse.
+      simpl. rewrite (eq_id _ X). auto. 
+      apply E_Ass_s. reflexivity.
+Qed.
+
+(** **** Exercise: 2 stars (ceval_example2)  *)
+Example ceval_example2:
+    (X ::= ANum 0;; Y ::= ANum 1;; Z ::= ANum 2) / empty_state ||
+    (update (update (update empty_state X 0) Y 1) Z 2).
+Proof.
+  (* FILL IN HERE *) 
+   apply E_Seq  with (update empty_state X 0).
+   Case "assignment x". 
+     apply E_Ass_s.  reflexivity. 
+   apply E_Seq  with (update (update empty_state X 0) Y 1).
+   Case "assignment y". 
+     apply E_Ass_s.  reflexivity. 
+   Case "assignment z". 
+     apply E_Ass_s.  reflexivity. 
+Qed.
+
+
+
+(* ####################################################### *)
+(** ** Determinism of Evaluation *)
+
+(** Changing from a computational to a relational definition of
+    evaluation is a good move because it allows us to escape from the
+    artificial requirement (imposed by Coq's restrictions on
+    [Fixpoint] definitions) that evaluation should be a total
+    function.  But it also raises a question: Is the second definition
+    of evaluation actually a partial function?  That is, is it
+    possible that, beginning from the same state [st], we could
+    evaluate some command [c] in different ways to reach two different
+    output states [st'] and [st'']?
+
+    In fact, this cannot happen: [ceval] is a partial function.
+    Here's the proof: *)
+
+(* <$Date: 2014-12-26 15:20:26 -0500 (Fri, 26 Dec 2014) $ *)
+
